proof/Base.v
@@ -1,6 +1,33 @@
 (* Basic definitions shared by all modules *)
 
-Require Export Cases.
+
+(* Cases library due to Aaron Bohannon ********************)
+Require String. Open Scope string_scope.
+
+Ltac move_to_top x :=
+  match reverse goal with
+  | H : _ |- _ => try move x after H
+  end.
+
+Tactic Notation "assert_eq" ident(x) constr(v) :=
+  let H := fresh in
+  assert (x = v) as H by reflexivity;
+  clear H.
+
+Tactic Notation "Case_aux" ident(x) constr(name) :=
+  first [
+    set (x := name); move_to_top x
+  | assert_eq x name; move_to_top x
+  | fail 1 "because we are working on a different case" ].
+
+Tactic Notation "Case" constr(name) := Case_aux Case name.
+Tactic Notation "SCase" constr(name) := Case_aux SCase name.
+Tactic Notation "SSCase" constr(name) := Case_aux SSCase name.
+Tactic Notation "SSSCase" constr(name) := Case_aux SSSCase name.
+Tactic Notation "SSSSCase" constr(name) := Case_aux SSSSCase name.
+Tactic Notation "SSSSSCase" constr(name) := Case_aux SSSSSCase name.
+Tactic Notation "SSSSSSCase" constr(name) := Case_aux SSSSSSCase name.
+Tactic Notation "SSSSSSSCase" constr(name) := Case_aux SSSSSSSCase name.
 
 
 (* bool ***************************************************)
@@ -27,6 +54,8 @@ Fixpoint beq_nat (n m : nat) : bool :=
  | S n1, S n2 => beq_nat n1 n2
  end.
 
+Hint Unfold beq_nat.
+
 
 Theorem beq_nat_refl
  : forall n : nat
@@ -43,7 +72,7 @@ Theorem beq_nat_sym
  : forall n1 n2 : nat
  , beq_nat n1 n2 = beq_nat n2 n1.
 Proof. 
- induction n1.
+  induction n1.
   intro n2. destruct n2.
    trivial.
    simpl. trivial.
@@ -62,7 +91,7 @@ Proof.
   destruct n2.
    simpl. auto.
    simpl. intro contra. inversion contra.
-  intro n2. destruct n2.
+   intro n2. destruct n2.
    simpl. intro contra. inversion contra.
    simpl. auto.
 Qed.
@@ -76,7 +105,7 @@ Proof.
   destruct n2.
    auto.
    simpl. intro. inversion H.
-  intro. destruct n2.
+   intro. destruct n2.
    simpl. intro. inversion H.
    simpl. intro. inversion H. apply beq_nat_refl.
 Qed.
@@ -109,5 +138,4 @@ Proof.
    intro. simpl. trivial.
    intro. simpl. apply IHn1. contradict H. subst. trivial.
 Qed.
-
 
