proof/Context.v
@@ -1,4 +1,5 @@
-(* typing contexts *)
+(* Typing contexts. *)
+
 Require Import Base.
 Require Import Name.
 Require Import FunctionalExtensionality.
@@ -20,8 +21,11 @@ Definition extend {A:Type} (rest:partial_map A) (x:name) (T:A)
        then some T
        else rest x'.
 
+Hint Unfold extend.
 
-(* An extended contexted contains the member we extended it with *)
+
+(* An extended contexted contains the member we extended it with. 
+ *)
 Lemma extend_eq 
  : forall A (ctx: partial_map A) x T
  , (extend ctx x T) x = some T.
@@ -30,8 +34,12 @@ Proof.
  rewrite <- beq_name_refl. trivial.
 Qed.
 
+Hint Resolve extend_eq.
 
-(* Skippin over members that don't match the name we care about *)
+
+(* We can skip over elements in a context that don't match 
+   then one we're looking for.
+ *)
 Lemma extend_neq
  :  forall A (ctx: partial_map A) x1 T x2
  ,  x2 <> x1
@@ -43,8 +51,12 @@ Proof.
  trivial.
 Qed.
 
+Hint Resolve extend_neq.
 
-(* Swap order of elements in context *)
+
+(* If two elements in a context are bound to different names, 
+   then we can swap their order. 
+ *)
 Lemma extend_swap
  :   forall A (ctx: partial_map A) x T1 y T2
  ,   x <> y
@@ -60,3 +72,5 @@ Proof.
   apply true_name_eq in Heqe2. subst. contradict H. trivial.
   trivial. trivial.
 Qed.
+
+Hint Resolve extend_swap.
