proof/Progress.v
@@ -1,88 +1,13 @@
 
 Require Import TyJudge.
 Require Import EvJudge.
-Require Import FunctionalExtensionality.
-
-Theorem closed_var_not
- : forall n
- , ~(closed (XVar n)).
-Proof.
- intro. unfold not. intro.
- unfold closed in H.
- specialize H with n. contradict H. apply FreeX_var.
-Qed.
 
 
-Theorem functional_extensionality_not
- : forall A B (f : A -> B) (g : A -> B)
- , (exists x, f x <> g x) -> f <> g.
-Proof.
- intros. unfold not. intro. subst.
- inversion H. contradiction H0.
- trivial.
-Qed.
-
-
-Theorem check_closed_in_empty
- : forall env t T 
- , closed t -> TYPE env t T -> TYPE empty t T.
-Proof.
- intros.
- eapply tyenv_invariance.
- apply H0.
- intros. contradict H1. unfold closed in H. apply H.
-Qed.
-
-
-Theorem closed_lam
- : forall x T t 
- , closed t -> closed (XLam x T t).
-Proof. 
- intros. unfold closed. intros. unfold not. intro.
- inversion H0. subst.
- unfold closed in H. apply H in H6. assumption.
-Qed.
-
-
-Theorem closed_app
- : forall t1 t2
- , closed t1 -> closed t2 -> closed (XApp t1 t2).
-Proof. 
- intros.
- unfold closed. intros. unfold not. intro.
- unfold closed in H.  specialize H  with x.
- unfold closed in H0. specialize H0 with x.
- inversion H1. subst. auto. subst. auto.
-Qed.
-
-
-Theorem check_empty_is_closed
- : forall t T
- , TYPE empty t T -> closed t.
-Proof.
- intros t T.
- generalize T.
- induction t.
- Case "XVar".
-  intros. inversion H. subst. unfold empty in H2. inversion H2.
- Case "XLam".
-  intros. inversion H. subst.
-  unfold closed. intro.
-  unfold not. intro.
-  eapply tyenv_contains_free_vars with (x:=x) in H.
-  inversion H. inversion H1. assumption.
- Case "XApp".
-  intros. inversion H. subst.
-  apply closed_app.
-  eapply IHt1. apply H3.
-  eapply IHt2. apply H5.
-Qed.
-
-
+(* A well typed term is either a value, or can transition to the next state. *)
 Theorem progress
  :  forall t T
  ,  TYPE  empty t T
- -> VALUE t \/ (exists t', STEP t t').
+ -> value t \/ (exists t', STEP t t').
 Proof.
  intros t T. intros Ht.
  remember (@empty ty) as G.
@@ -90,7 +15,7 @@ Proof.
  Case "XVar".
   left. subst. inversion H. subst.
  Case "XLam".
-  left. apply VALUE_XLam.
+  left. apply Value_lam.
   apply TYLam in Ht.
   eapply check_empty_is_closed. apply Ht.
  Case "XApp".
@@ -103,7 +28,7 @@ Proof.
    SSCase "t2 steps".
     destruct H0 as [t2' Htsp].
     exists (XApp (XLam x T t) t2').
-    apply EVApp2. apply VALUE_XLam. assumption. assumption.
+    apply EVApp2. apply Value_lam. assumption. assumption.
   SCase "t1 steps".
    destruct H as [t1' Htsp].
    exists (XApp t1' t2).
